cleanup: new def of strlen, attempt of lbody function

c/poc/strlen_spec.v
@@ -86,98 +86,66 @@ Inductive strlen_mem_op : mem -> block -> Z -> option (C_string*nat) -> Prop :=
 | LengthSuccMem_op : forall m b ofs c s n, strlen_mem_op m b (ofs + 1) (Some (s,n)) -> Mem.load Mint8signed m b ofs = Some (VintP c) -> strlen_mem_op m b ofs (Some ((CString c s),(S n))).
 
 Inductive strlen_mem : mem -> block -> Z -> nat -> Prop :=
-| LengthZeroMem m b ofs: Mem.load Mint8signed m b ofs = Some (VintZ 0) -> strlen_mem m b ofs 0
+| LengthZeroMem m b ofs: Mem.load Mint8unsigned m b ofs = Some (VintZ 0) -> strlen_mem m b ofs 0
 | LengthSuccMem m b ofs: forall p v,
     strlen_mem m b (ofs+1) p ->
-    Mem.load Mint8signed m b ofs = Some (VintP v) ->
+    Mem.load Mint8unsigned m b ofs = Some (VintP v) ->
     strlen_mem m b ofs (S p).
 
 (* strlen C light AST *)
 
-Definition _i : ident := 54%positive.
-Definition _s : ident := 53%positive.
-Definition _strlen : ident := 55%positive.
-
-Notation _input := _s.
-Notation _output := _i.
+Definition _output : ident := 4%positive.
+Definition _input : ident := 3%positive.
+Definition _t'1 : ident := 7%positive.
+Definition _t'2 : ident := 8%positive.
 
 Definition f_strlen := {|
   fn_return := tuint;
   fn_callconv := cc_default;
-  fn_params := ((_s, (tptr tschar)) :: nil);
+  fn_params := ((_input, (tptr tuchar)) :: nil);
   fn_vars := nil;
-  fn_temps := ((_i, tuint) :: nil);
+  fn_temps := ((_output, tuint) :: (_t'1, (tptr tuchar)) :: (_t'2, tuchar) :: nil);
   fn_body :=
 (Ssequence
+  (Sset _output (Econst_int (Int.repr 0) tint))
   (Ssequence
-    (Sset _i (Econst_int (Int.repr 0) tint))
     (Sloop
-      (Sifthenelse (Ebinop One
-                     (Ederef
-                       (Ebinop Oadd (Etempvar _s (tptr tschar))
-                         (Etempvar _i tuint) (tptr tschar)) tschar)
-                     (Econst_int (Int.repr 0) tint) tint)
-        Sskip
-        Sbreak)
-      (Sset _i
-        (Ebinop Oadd (Etempvar _i tuint) (Econst_int (Int.repr 1) tint)
-          tuint))))
-  (Sreturn (Some (Etempvar _i tuint))))
-                      |}.
+      (Ssequence
+        (Ssequence
+          (Ssequence
+            (Sset _t'1 (Etempvar _input (tptr tuchar)))
+            (Sset _input
+              (Ebinop Oadd (Etempvar _t'1 (tptr tuchar))
+                (Econst_int (Int.repr 1) tint) (tptr tuchar))))
+          (Ssequence
+            (Sset _t'2 (Ederef (Etempvar _t'1 (tptr tuchar)) tuchar))
+            (Sifthenelse (Etempvar _t'2 tuchar) Sskip Sbreak)))
+        (Sset _output
+          (Ebinop Oadd (Etempvar _output tuint) (Econst_int (Int.repr 1) tint)
+            tuint)))
+      Sskip)
+    (Sreturn (Some (Etempvar _output tuint)))))
+                          |}.
 
-
-(* Loop of f_strlen *)
-
-Definition f_strlen_loop :=  (Sloop
-      (Sifthenelse (Ebinop One (* comparison ([!=]) *)
-                     (Ederef (* pointer dereference (unary [*]) *)
-                       (Ebinop Oadd (Etempvar _input (tptr tschar))
-                         (Etempvar _output tuint) (tptr tschar)) tschar)
-                     (Econst_int (Int.repr 0) tint) tint)
-        Sskip
-        Sbreak)
-      (Sset _output
-        (Ebinop Oadd (Etempvar _output tuint) (Econst_int (Int.repr 1) tint)
-                tuint))).
+Definition f_strlen_loop :=
+  (Sloop
+      (Ssequence
+        (Ssequence
+          (Ssequence
+            (Sset _t'1 (Etempvar _input (tptr tuchar)))
+            (Sset _input
+              (Ebinop Oadd (Etempvar _t'1 (tptr tuchar))
+                (Econst_int (Int.repr 1) tint) (tptr tuchar))))
+          (Ssequence
+            (Sset _t'2 (Ederef (Etempvar _t'1 (tptr tuchar)) tuchar))
+            (Sifthenelse (Etempvar _t'2 tuchar) Sskip Sbreak)))
+        (Sset _output
+          (Ebinop Oadd (Etempvar _output tuint) (Econst_int (Int.repr 1) tint)
+            tuint)))
+      Sskip).
 
 (* Correctness statements *)
-
-(* On empty string then C light function evaluates to 0 *)
-Lemma strlen_correct_empty_string :
-  (* with this assumption Ptrofs.modulus = Int.modulus, ptherwise Ptrofs.modulus > Int.modulus *)
-  Archi.ptr64 = false ->
-  forall ge e m b ofs le len,                       
-    (* Preconditions on the length of the string and valid offset *)
-    0 < ofs < Ptrofs.modulus ->
-    Z_of_nat len < Int.modulus ->
-    ofs + Z_of_nat len < Ptrofs.modulus ->                      
-    (* Initialize local variables *)
-    le!_input = Some (Vptr b (Ptrofs.repr ofs)) ->
-    le!_output = Some (VintZ 0) ->                     
-    (* Precondition: reading empty C string from memory *)
-    strlen_mem m b ofs O ->
-    (* C light expression f_strlen returns O and assigns O to output variable *)
-    exists t le', exec_stmt ge e le m f_strlen.(fn_body) t le' m (Out_return (Some ((VintN O),tuint))) /\ (le'!_output) = Some (VintN O).
-Proof.
-  intros.
-  inversion H5.
-  repeat eexists.
-  - seq1.
-    + seq1.
-      * sset. (* evaluate expression *) repeat econstructor.
-      * eapply exec_Sloop_stop1. (* break from the loop *)
-        repeat econstructor. repeat gso_assumption. 
-        eapply gss. 
-        repeat econstructor. simpl.
-        replace (Ptrofs.unsigned
-                   (Ptrofs.add (Ptrofs.repr ofs) (Ptrofs.mul (Ptrofs.repr 1) (Ptrofs.of_intu (Int.repr 0))))) with ofs. apply H6.
-        { pose (Ptrofs.modulus_eq32 H). ptrofs_compute_add_mul. all: nia. }
-        repeat econstructor. simpl. repeat econstructor. econstructor. econstructor.
-    + (* return statement *)
-      repeat econstructor. eapply gss.
-  - eapply gss.
-Qed.
-
+(* On empty string C light function evaluates to 0 *)
 
 Lemma strlen_correct_loop_empty_string :
   (* with this assumption Ptrofs.modulus = Int.modulus, ptherwise Ptrofs.modulus > Int.modulus *)
@@ -193,158 +161,27 @@ Lemma strlen_correct_loop_empty_string :
     (* Precondition: reading empty C string from memory *)
     strlen_mem m b ofs O ->
     (* C light expression f_strlen returns O and assigns O to output variable *)
-    exists t le', exec_stmt ge e le m f_strlen_loop t le' m Out_normal /\ (le'!_output) = Some (VintN O).
+    exists t le', exec_stmt ge e le m f_strlen_loop t le' m Out_normal /\ le'!_output = Some (VintZ 0).
 Proof.
   intros.
   inversion_clear H5.
   repeat eexists.
-  - eapply exec_Sloop_stop1. (* break from the loop *)
-    repeat econstructor. 1,2: gso_assumption.
-    repeat econstructor. simpl.
-    replace (Ptrofs.unsigned
-               (Ptrofs.add (Ptrofs.repr ofs) (Ptrofs.mul (Ptrofs.repr 1) (Ptrofs.of_intu (Int.repr 0))))) with ofs.  apply H6. { pose (Ptrofs.modulus_eq32 H). ptrofs_compute_add_mul. all: nia. }
-   repeat econstructor. simpl. repeat econstructor. econstructor. econstructor.    
-  - assumption.
+  eapply exec_Sloop_stop1.
+  seq2. repeat econstructor. gso_assumption. apply gss.
+  repeat econstructor. rewrite gso. apply gss. cbv; congruence. simpl.
+  replace (Ptrofs.unsigned (Ptrofs.repr ofs)) with ofs. 
+  apply H6.
+  { pose (Ptrofs.modulus_eq32 H). ptrofs_compute_add_mul. all: nia. }
+  apply gss. econstructor.
+  replace (negb (Int.eq (Int.repr 0) Int.zero)) with false by simpl.
+  econstructor.
+  cbv; congruence.
+  econstructor.
+  repeat (rewrite gso). assumption. all: cbv; congruence.
 Qed.
 
 
-Lemma strlen_correct_loop_empty_string1 :
-  (* with this assumption Ptrofs.modulus = Int.modulus, ptherwise Ptrofs.modulus > Int.modulus *)
-  Archi.ptr64 = false ->
-  forall ge e m b ofs le len,                       
-    (* Preconditions on the length of the string and valid offset *)
-    0 < ofs < Ptrofs.modulus ->
-    Z_of_nat len < Int.modulus ->
-    ofs + Z_of_nat len < Ptrofs.modulus ->                      
-    (* Initialize local variables *)
-    le!_input = Some (Vptr b (Ptrofs.repr ofs)) ->
-    le!_output = Some (VintZ 0) ->                     
-    (* Precondition: reading empty C string from memory *)
-    strlen_mem m b ofs O ->
-    (* C light expression f_strlen returns O and assigns O to output variable *)
-    exists t, exec_stmt ge e le m f_strlen_loop t le m Out_normal.
-Proof.
-  intros.
-  inversion_clear H5.
-   eexists.
-  - eapply exec_Sloop_stop1. (* break from the loop *)
-    repeat econstructor. 1,2: gso_assumption.
-    repeat econstructor. simpl.
-    replace (Ptrofs.unsigned
-               (Ptrofs.add (Ptrofs.repr ofs) (Ptrofs.mul (Ptrofs.repr 1) (Ptrofs.of_intu (Int.repr 0))))) with ofs. apply H6. { pose (Ptrofs.modulus_eq32 H). ptrofs_compute_add_mul. all: nia. }
-   repeat econstructor. simpl. repeat econstructor. econstructor. econstructor.    
-
-Qed.
-
- 
-(* Conditions about the f_strlen loop *)
-
-(* If 0 is read from memory at [b,ofs + len] the output is set to len *)
-Lemma strlen_loop_break_correct : Archi.ptr64 = false -> forall ge e m b ofs outp le,
-      ofs + Z.of_nat outp < Ptrofs.modulus ->
-      0 < ofs < Ptrofs.modulus ->
-      0 <= Z.of_nat outp < Ptrofs.modulus ->
-      le!_input = Some (Vptr b (Ptrofs.repr ofs)) ->
-      le!_output = Some (VintN outp) -> 
-      Mem.load Mint8signed m b (ofs + (Z_of_nat outp)) = Some (Vint (Int.repr 0)) ->
-      exists t le', exec_stmt ge e le m f_strlen_loop t le' m Out_normal /\
-        (le'!_output) = Some (VintN outp).
-Proof.
-  intros.
-  repeat eexists.
-  - eapply exec_Sloop_stop1.
-    repeat econstructor; repeat gso_assumption. 
-    repeat econstructor. simpl.
-    replace (Ptrofs.unsigned
-       (Ptrofs.add (Ptrofs.repr ofs)
-                   (Ptrofs.mul (Ptrofs.repr 1) (Ptrofs.of_intu (Int.repr (Z.of_nat outp)))))) with (ofs + (Z_of_nat outp)). apply H5.
-        { pose (Ptrofs.modulus_eq32 H). ptrofs_compute_add_mul. all: nia. }
-        repeat econstructor. simpl. repeat econstructor. econstructor. econstructor.
-  - assumption.
-Qed.
-
-Lemma strlen_loop_break_correct1 : Archi.ptr64 = false -> forall ge e m b ofs outp le,
-      ofs + Z.of_nat outp < Ptrofs.modulus ->
-      0 < ofs < Ptrofs.modulus ->
-      0 <= Z.of_nat outp < Ptrofs.modulus ->
-      le!_input = Some (Vptr b (Ptrofs.repr ofs)) ->
-      le!_output = Some (VintN outp) ->
-      Mem.load Mint8signed m b (ofs + (Z_of_nat outp)) = Some (Vint (Int.repr 0)) ->
-      exists t, exec_stmt ge e le m f_strlen_loop t le m Out_normal.
-Proof.
-   intros.
-  repeat eexists.
-  - eapply exec_Sloop_stop1.
-    repeat econstructor; repeat gso_assumption. 
-    repeat econstructor. simpl.
-    replace (Ptrofs.unsigned
-       (Ptrofs.add (Ptrofs.repr ofs)
-                   (Ptrofs.mul (Ptrofs.repr 1) (Ptrofs.of_intu (Int.repr (Z.of_nat outp)))))) with (ofs + (Z_of_nat outp)). apply H5.
-        { pose (Ptrofs.modulus_eq32 H). ptrofs_compute_add_mul. all: nia. }
-        repeat econstructor. simpl. repeat econstructor. econstructor. econstructor.
-Qed.
-
-
-Definition _out : ident := 4%positive.
-Definition _main : ident := 6%positive.
-Definition _in : ident := 3%positive.
-Definition _t'1 : ident := 7%positive.
-Definition _t'2 : ident := 8%positive.
-
-Definition f_strlen_new := {|
-  fn_return := tuint;
-  fn_callconv := cc_default;
-  fn_params := ((_in, (tptr tuchar)) :: nil);
-  fn_vars := nil;
-  fn_temps := ((_out, tuint) :: (_t'1, (tptr tuchar)) :: (_t'2, tuchar) :: nil);
-  fn_body :=
-(Ssequence
-  (Sset _out (Econst_int (Int.repr 0) tint))
-  (Ssequence
-    (Sloop
-      (Ssequence
-        (Ssequence
-          (Ssequence
-            (Sset _t'1 (Etempvar _in (tptr tuchar)))
-            (Sset _in
-              (Ebinop Oadd (Etempvar _t'1 (tptr tuchar))
-                (Econst_int (Int.repr 1) tint) (tptr tuchar))))
-          (Ssequence
-            (Sset _t'2 (Ederef (Etempvar _t'1 (tptr tuchar)) tuchar))
-            (Sifthenelse (Etempvar _t'2 tuchar) Sskip Sbreak)))
-        (Sset _out
-          (Ebinop Oadd (Etempvar _out tuint) (Econst_int (Int.repr 1) tint)
-            tuint)))
-      Sskip)
-    (Sreturn (Some (Etempvar _out tuint)))))
-                          |}.
-
-Definition f_strlen_loop_new :=
-  (Sloop
-      (Ssequence
-        (Ssequence
-          (Ssequence
-            (Sset _t'1 (Etempvar _in (tptr tuchar)))
-            (Sset _in
-              (Ebinop Oadd (Etempvar _t'1 (tptr tuchar))
-                (Econst_int (Int.repr 1) tint) (tptr tuchar))))
-          (Ssequence
-            (Sset _t'2 (Ederef (Etempvar _t'1 (tptr tuchar)) tuchar))
-            (Sifthenelse (Etempvar _t'2 tuchar) Sskip Sbreak)))
-        (Sset _out
-          (Ebinop Oadd (Etempvar _out tuint) (Econst_int (Int.repr 1) tint)
-            tuint)))
-      Sskip).
-
-Inductive strlen_mem_u : mem -> block -> Z -> nat -> Prop :=
-| LengthZeroMemu m b ofs: Mem.load Mint8unsigned m b ofs = Some (VintZ 0) -> strlen_mem_u m b ofs 0
-| LengthSuccMemu m b ofs: forall p v,
-    strlen_mem_u m b (ofs+1) p ->
-    Mem.load Mint8unsigned m b ofs = Some (VintP v) ->
-    strlen_mem_u m b ofs (S p).
-
-
-(* On a string of length 2 C light function evaluates to 0 *)
+(* Test case: On a string of length 2 C light function evaluates to 0 *)
 Lemma strlen_correct_test :
   (* with this assumption Ptrofs.modulus = Int.modulus, ptherwise Ptrofs.modulus > Int.modulus *)
   Archi.ptr64 = false ->
@@ -354,13 +191,13 @@ Lemma strlen_correct_test :
     Z_of_nat len < Int.modulus ->
     ofs + Z_of_nat len < Ptrofs.modulus ->                      
     (* Initialize local variables *)
-    le!_in = Some (Vptr b (Ptrofs.repr ofs)) ->
-    le!_out = Some (VintZ 0) ->                     
+    le!_input = Some (Vptr b (Ptrofs.repr ofs)) ->
+    le!_output = Some (VintZ 0) ->                     
     (* Precondition: reading  C string of length 2 from memory *)
-    strlen_mem_u m b ofs 2%nat ->
+    strlen_mem m b ofs 2%nat ->
     
     (* C light expression f_strlen returns O and assigns O to output variable *)
-    exists t le', exec_stmt ge e le m f_strlen_new.(fn_body) t le' m (Out_return (Some ((VintZ 2),tuint))) /\ (le'!_out) = Some (VintZ 2).
+    exists t le', exec_stmt ge e le m f_strlen.(fn_body) t le' m (Out_return (Some ((VintZ 2),tuint))) /\ (le'!_output) = Some (VintZ 2).
 Proof.
   intros.
   inversion_clear H5. inversion_clear H6. inversion_clear H5.
@@ -380,7 +217,7 @@ Proof.
         rewrite gso. rewrite gso. rewrite gso. apply gss. 1-3: cbv ;congruence.
         repeat econstructor. econstructor. econstructor.
 
-        (* loop 1 *)
+        (* loop 2 *)
         loop. repeat econstructor. repeat gso_assumption.
         rewrite gso. rewrite gso. apply gss. 1-2: cbv ; congruence.
         apply gss.
@@ -400,8 +237,6 @@ Proof.
             
          (* exit loop *)
         eapply exec_Sloop_stop1.
-        Print exec_stmt.
-        (* break from the loop *)
         seq2. seq1. seq1. econstructor. econstructor. rewrite gso. rewrite gso. apply gss. 1-2: cbv ; congruence.
         repeat econstructor.
         apply gss.
@@ -428,93 +263,92 @@ Proof.
   - rewrite gso.  rewrite gso.  rewrite gso.  eapply gss. all: cbv ; congruence.
 Admitted.
 
-(* Some tests *)
+(* Conditions about the f_strlen loop *)
 
-(* On a string of length 2 C light function evaluates to 0 *)
-Lemma strlen_correct_test_old :
-  (* with this assumption Ptrofs.modulus = Int.modulus, ptherwise Ptrofs.modulus > Int.modulus *)
-  Archi.ptr64 = false ->
-  forall ge e m b ofs le len,                       
-    (* Preconditions on the length of the string and valid offset *)
-    0 < ofs < Ptrofs.modulus ->
-    Z_of_nat len < Int.modulus ->
-    ofs + Z_of_nat len < Ptrofs.modulus ->                      
-    (* Initialize local variables *)
-    le!_input = Some (Vptr b (Ptrofs.repr ofs)) ->
-    le!_output = Some (VintZ 0) ->                     
-    (* Precondition: reading  C string of length 2 from memory *)
-    strlen_mem m b ofs 2%nat ->
-    
-    (* C light expression f_strlen returns O and assigns O to output variable *)
-    exists t le', exec_stmt ge e le m f_strlen.(fn_body) t le' m (Out_return (Some ((VintZ 2),tuint))) /\ (le'!_output) = Some (VintZ 2).
+(* If 0 is read from memory at [b,ofs + len] the output is set to len *)
+Lemma strlen_loop_break_correct : Archi.ptr64 = false -> forall ge e m b ofs outp le,
+      
+      ofs + Z.of_nat outp < Ptrofs.modulus ->
+      0 < ofs < Ptrofs.modulus ->
+      0 <= Z.of_nat outp < Ptrofs.modulus ->
+
+      (* IF before the loop *s = [b,ofs + outp] and i = outp *)
+      le!_input = Some (Vptr b (Ptrofs.repr (ofs + Z.of_nat outp))) ->
+      le!_output = Some (VintN outp) ->
+      
+      (* and the guard condition is false *)
+      Mem.load Mint8unsigned m b (ofs + (Z_of_nat outp)) = Some (Vint (Int.repr 0)) ->
+
+      (* THEN loop executes to an environment with i = outp [i.e., i stays unchanged] + memory is unchanged *)
+      exists t le', exec_stmt ge e le m f_strlen_loop t le' m Out_normal /\ (le'!_output) = Some (VintN outp).
 Proof.
   intros.
-  inversion_clear H5. inversion_clear H6. inversion_clear H5.
   repeat eexists.
-  - seq1.
-    + seq1.
-      * sset. (* evaluate expression *) repeat econstructor.
-      * (* loop 1 *)
-        loop. repeat econstructor. repeat gso_assumption. eapply gss.        repeat econstructor. simpl. replace (Ptrofs.unsigned (Ptrofs.add (Ptrofs.repr ofs) (Ptrofs.mul (Ptrofs.repr 1) (Ptrofs.of_intu (Int.repr 0))))) with ofs. apply H7.  { pose (Ptrofs.modulus_eq32 H). ptrofs_compute_add_mul. all: nia. } repeat econstructor. simpl. repeat econstructor. simpl.
-        replace (negb (Int.eq (Int.repr (Z.pos v)) (Int.repr 0))) with true.      
-        econstructor. admit. repeat econstructor. repeat econstructor. repeat econstructor. apply gss. repeat econstructor.
-
-        (* loop 2 *)
-        loop. repeat econstructor. rewrite gso; repeat gso_assumption. eapply gss.
-        repeat econstructor. simpl. replace (Ptrofs.unsigned
-       (Ptrofs.add (Ptrofs.repr ofs)
-                   (Ptrofs.mul (Ptrofs.repr 1) (Ptrofs.of_intu (Int.add (Int.repr 0) (Int.repr 1)))))) with (ofs + 1). apply H8.  { pose (Ptrofs.modulus_eq32 H). ptrofs_compute_add_mul. all: admit. }        repeat econstructor. simpl. repeat econstructor. simpl.
-        replace (negb (Int.eq (Int.repr (Z.pos v0)) (Int.repr 0))) with true.
-      
-        econstructor. repeat econstructor. repeat econstructor. admit.  econstructor. repeat econstructor. repeat econstructor. apply gss. repeat econstructor.
-         (* exit loop *)
-        eapply exec_Sloop_stop1. (* break from the loop *)
-        repeat econstructor.  rewrite gso; repeat gso_assumption.  rewrite gso; repeat gso_assumption.  eapply gss.
-        repeat econstructor. simpl.
-        replace  (Ptrofs.unsigned
-       (Ptrofs.add (Ptrofs.repr ofs)
-          (Ptrofs.mul (Ptrofs.repr 1)
-             (Ptrofs.of_intu (Int.add (Int.add (Int.repr 0) (Int.repr 1)) (Int.repr 1)))))) with (ofs + 2). replace (ofs + 2) with (ofs + 1 + 1) by lia. apply H6. { admit. }
-        repeat econstructor. simpl. repeat econstructor. econstructor. econstructor.
-    + (* return statement *)
-      repeat econstructor. eapply gss.
-  - eapply gss.
+  eapply exec_Sloop_stop1.
+  seq2. seq1. seq1.
+  repeat econstructor.
+  apply H3.
+  repeat econstructor.
+  apply gss.
+  repeat econstructor.
+  seq1.
+  repeat econstructor.
+  rewrite gso. apply gss. cbv ; congruence.
+  unfold Mem.loadv.
+  replace (Ptrofs.unsigned (Ptrofs.repr (ofs + Z.of_nat outp))) with (ofs + Z.of_nat outp) by admit.
+  apply H5.
+  repeat econstructor.
+  apply gss.
+  econstructor.
+  replace (negb (Int.eq (Int.repr 0) Int.zero)) with false by (simpl).
+  econstructor.
+  cbv; congruence.
+  econstructor.
+  repeat (rewrite gso). assumption.
+  all: cbv; congruence.
 Admitted.
 
 
-Lemma strlen_correct_loop_empty_string_new :
-  (* with this assumption Ptrofs.modulus = Int.modulus, ptherwise Ptrofs.modulus > Int.modulus *)
-  Archi.ptr64 = false ->
-  forall ge e m b ofs le len,                       
-    (* Preconditions on the length of the string and valid offset *)
-    0 < ofs < Ptrofs.modulus ->
-    Z_of_nat len < Int.modulus ->
-    ofs + Z_of_nat len < Ptrofs.modulus ->                      
-    (* Initialize local variables *)
-    le!_in = Some (Vptr b (Ptrofs.repr ofs)) ->
-    le!_out = Some (VintZ 0) ->                     
-    (* Precondition: reading empty C string from memory *)
-    strlen_mem_u m b ofs O ->
-    (* C light expression f_strlen returns O and assigns O to output variable *)
-    exists t le', exec_stmt ge e le m f_strlen_loop_new t le' m Out_normal.
+(* Helper lemmas about strlen_mem *)
+
+Lemma strlen_trans_len_0 : forall len m b ofs, strlen_mem m b ofs len -> strlen_mem m b (ofs + Z.of_nat len) O.
 Proof.
-  intros.
-  inversion_clear H5.
-  repeat eexists.
-  eapply exec_Sloop_stop1.
-  seq2. repeat econstructor. gso_assumption. apply gss.
-  repeat econstructor. rewrite gso. apply gss. cbv; congruence. simpl.
-  replace (Ptrofs.unsigned (Ptrofs.repr ofs)) with ofs. 
-  apply H6.
-  { pose (Ptrofs.modulus_eq32 H). ptrofs_compute_add_mul. all: nia. }
-  apply gss. econstructor.
-  replace (negb (Int.eq (Int.repr 0) Int.zero)) with false by simpl.
-  econstructor.
-  cbv; congruence.
-  econstructor.    
+  induction len ; intros.
+  - replace (ofs + Z.of_nat 0) with ofs by nia. assumption.
+  - inversion_clear H.
+    replace (ofs + Z.of_nat (S len)) with (ofs + 1 + Z.of_nat len) by nia.
+    apply (IHlen m b (ofs + 1) H0).
 Qed.
 
-(*Lemma strlen_loop_correct_new : (* with this assumption Ptrofs.modulus = Int.modulus, ptherwise Ptrofs.modulus > Int.modulus *)
+Lemma strlen_trans_len_i : forall len m b ofs, strlen_mem m b ofs len -> forall i, (i < len)%nat -> strlen_mem m b (ofs + Z.of_nat i) (len - i)%nat.
+Proof.
+  induction len.
+  - intros. omega.
+  - induction i ; intro.
+    + replace (ofs + Z.of_nat 0) with ofs by nia.
+       replace  (S len - 0)%nat with (S len)%nat by omega. assumption. 
+    + inversion_clear H.
+       assert (i < len)%nat by omega. pose (IHlen m b (ofs + 1) H1 i H).
+       replace (S len - S i)%nat with (len - i)%nat by omega.
+       replace (ofs + Z.of_nat (S i)) with  (ofs + 1 + Z.of_nat i) by nia.
+       assumption.
+Qed.  
+   
+Lemma strlen_to_mem : forall len m b ofs, strlen_mem m b ofs len ->
+                                     forall i, (i < len)%nat -> exists p : positive, Mem.load chunk m b (ofs + Z.of_nat i) = Some (VintP p).
+Proof.
+  induction len.
+  - intros. omega.
+  -  induction i ; intro ; inversion_clear H.
+    +  replace (ofs + Z.of_nat 0) with ofs by nia.
+       exists v. assumption.
+    +  assert (i < len)%nat by omega. pose (IHlen m b (ofs + 1) H1 i H).
+       replace (ofs + Z.of_nat (S i)) with  (ofs + 1 + Z.of_nat i) by nia.
+       assumption.  
+Qed.
+
+
+Lemma strlen_loop_continue_correct : (* with this assumption Ptrofs.modulus = Int.modulus, otherwise Ptrofs.modulus > Int.modulus *)
   Archi.ptr64 = false ->
   forall len ge e m b ofs le,
                        
@@ -523,9 +357,101 @@ Qed.
     Z_of_nat len < Int.modulus ->
     ofs + Z_of_nat len < Ptrofs.modulus ->
                        
-                       (* Initialize local variables *)
-    le!_in = Some (Vptr b (Ptrofs.repr ofs)) ->
-    le!_out = Some (VintZ 0) ->
+    (* Initialize local variables *)
+    le!_input = Some (Vptr b (Ptrofs.repr (ofs + Z.of_nat len))) ->
+    le!_output = Some (VintN len) ->
+    
+     (* Memory reads *)
+      (exists p, Mem.load chunk m b (ofs + Z.of_nat len) = Some (VintP p)) ->
+                                         
+      exists t lef, exec_stmt ge e le m f_strlen_loop t lef m Out_normal ->  exists t les, exec_stmt ge e les m f_strlen_loop t lef m Out_normal /\ les!_output = Some (VintN (S len)).
+Proof.
+  intros.
+  destruct H5 as [p].
+  eexists.
+  eexists.
+  intro.
+  eexists.
+  exists (PTree.set _output
+       (Vint (Int.add (Int.repr (Z.of_nat len)) (Int.repr 1)))
+       (PTree.set _t'2 (VintP p)
+          (PTree.set _input
+             (Vptr b
+                (Ptrofs.add (Ptrofs.repr (ofs + Z.of_nat len))
+                   (Ptrofs.mul
+                      (Ptrofs.repr (sizeof ge tuchar))
+                      (ptrofs_of_int Signed (Int.repr 1)))))
+             (PTree.set _t'1
+                        (Vptr b (Ptrofs.repr (ofs + Z.of_nat len))) le)))).
+  split.
+  - solve_by_inverts 5%nat.  solve_by_inverts 5%nat. 
+  repeat eexists.
+(*   exists t lef, exec_stmt ge e le m f_strlen_loop t lef m Out_normal ->  exists t les, exec_stmt ge e les m f_strlen_loop t lef m Out_normal /\ les!_output = Some (VintN (S len)). *)
+
+Lemma strlen_loop_continue_correct : (* with this assumption Ptrofs.modulus = Int.modulus, otherwise Ptrofs.modulus > Int.modulus *)
+  Archi.ptr64 = false ->
+  forall len ge e m b ofs le,
+                       
+    (* Preconditions on the length of the string and valid offset *)
+    0 <= ofs < Ptrofs.modulus ->
+    Z_of_nat len < Int.modulus ->
+    ofs + Z_of_nat len < Ptrofs.modulus ->
+                       
+    (* Initialize local variables *)
+    le!_input = Some (Vptr b (Ptrofs.repr (ofs + Z.of_nat len))) ->
+    le!_output = Some (VintN len) ->
+    
+     (* Memory reads *)
+      (exists p, Mem.load chunk m b (ofs + Z.of_nat len) = Some (VintP p)) ->
+                                         
+      exists t le', exec_stmt ge e le m f_strlen_loop t le' m Out_normal /\ le'!_output = Some (VintN (S len)).
+Proof.
+  intros.
+  destruct H5 as [p].
+  (* (PTree.set _output
+       (Vint (Int.add (Int.repr (Z.of_nat len)) (Int.repr 1)))
+       (PTree.set _t'2 (VintP p)
+          (PTree.set _input
+             (Vptr b
+                (Ptrofs.add (Ptrofs.repr (ofs + Z.of_nat len))
+                   (Ptrofs.mul
+                      (Ptrofs.repr (sizeof ge tuchar))
+                      (ptrofs_of_int Signed (Int.repr 1)))))
+             (PTree.set _t'1
+                (Vptr b (Ptrofs.repr (ofs + Z.of_nat len))) le))))*)
+  repeat eexists.
+  loop. repeat econstructor. repeat gso_assumption. eapply gss. repeat econstructor.
+  rewrite gso. apply gss. cbv; congruence. simpl. ptrofs_to_Z. apply H5. lia.  
+  apply gss.
+  simpl.
+  econstructor.
+  replace (negb (Int.eq (Int.repr (Z.pos p)) Int.zero)) with true by admit.      
+  econstructor.
+  repeat (rewrite gso).
+  apply H4. 1-3: cbv; congruence.
+  repeat econstructor.
+  econstructor.
+  econstructor.
+  loop.
+  repeat econstructor.
+  Print exec_stmt.
+  
+  rewrite gso. rewrite gso. apply gss. 1-3: cbv ;congruence.
+  repeat econstructor. econstructor. econstructor.
+  
+  
+Lemma strlen_loop_correct : (* with this assumption Ptrofs.modulus = Int.modulus, otherwise Ptrofs.modulus > Int.modulus *)
+  Archi.ptr64 = false ->
+  forall len ge e m b ofs le,
+                       
+    (* Preconditions on the length of the string and valid offset *)
+    0 <= ofs < Ptrofs.modulus ->
+    Z_of_nat len < Int.modulus ->
+    ofs + Z_of_nat len < Ptrofs.modulus ->
+                       
+    (* Initialize local variables *)
+    le!_input = Some (Vptr b (Ptrofs.repr ofs)) ->
+    le!_output = Some (VintZ len) ->
     
      (* Memory reads *)
     (forall i, (i < len)%nat ->
@@ -601,45 +527,6 @@ Proof.
   inversion_clear H5.
       assumption. 
 Admitted. *)
-
-
-(* Helper lemmas about strlen_mem *)
-
-Lemma strlen_trans1 : forall len m b ofs, strlen_mem m b ofs len -> strlen_mem m b (ofs + Z.of_nat len) O.
-Proof.
-  induction len ; intros.
-  - replace (ofs + Z.of_nat 0) with ofs by nia. assumption.
-  - inversion_clear H.
-    replace (ofs + Z.of_nat (S len)) with (ofs + 1 + Z.of_nat len) by nia.
-    apply (IHlen m b (ofs + 1) H0).
-Qed.
-
-Lemma strlen_trans3 : forall len m b ofs, strlen_mem m b ofs len -> forall i, (i < len)%nat -> strlen_mem m b (ofs + Z.of_nat i) (len - i)%nat.
-Proof.
-  induction len.
-  - intros. omega.
-  - induction i ; intro.
-    + replace (ofs + Z.of_nat 0) with ofs by nia.
-       replace  (S len - 0)%nat with (S len)%nat by omega. assumption. 
-    + inversion_clear H.
-       assert (i < len)%nat by omega. pose (IHlen m b (ofs + 1) H1 i H).
-       replace (S len - S i)%nat with (len - i)%nat by omega.
-       replace (ofs + Z.of_nat (S i)) with  (ofs + 1 + Z.of_nat i) by nia.
-       assumption.
-Qed.  
-   
-Lemma strlen_trans4 : forall len m b ofs, strlen_mem_u m b ofs len ->
-                                     forall i, (i < len)%nat -> exists p : positive, Mem.load chunk m b (ofs + Z.of_nat i) = Some (VintP p).
-Proof.
-  induction len.
-  - intros. omega.
-  -  induction i ; intro ; inversion_clear H.
-    +  replace (ofs + Z.of_nat 0) with ofs by nia.
-       exists v. assumption.
-    +  assert (i < len)%nat by omega. pose (IHlen m b (ofs + 1) H1 i H).
-       replace (ofs + Z.of_nat (S i)) with  (ofs + 1 + Z.of_nat i) by nia.
-       assumption.  
-Qed.
 
 Lemma strlen_loop_correct : (* with this assumption Ptrofs.modulus = Int.modulus, ptherwise Ptrofs.modulus > Int.modulus *)
   Archi.ptr64 = false ->
